2-cyclic inductive done and security over the first machine proven

internship_machine.thy
@@ -106,7 +106,45 @@ lemma bigger_fish: "\<forall>q\<in>paths. \<forall>m. \<exists>n>m. \<exists>s_0
 definition cyclic_paths:: "(nat \<Rightarrow> STEP) set" where
 "cyclic_paths \<equiv> {q::(nat\<Rightarrow>STEP). q \<in> paths \<and> ( \<exists>n. \<exists>m. STATE(q n) = STATE(q m))}"
 
+inductive two_cyclic_path:: "(nat \<Rightarrow> STEP) \<Rightarrow> bool" where
+"\<forall>p \<in> paths. \<forall>n. INPUT(p n) = 1 \<Longrightarrow> two_cyclic_path p"
 
+definition two_cyclic_set :: "(nat \<Rightarrow> STEP) set" where
+"two_cyclic_set \<equiv> {p::(nat \<Rightarrow> STEP). two_cyclic_path p}"
+
+
+
+lemma "\<forall>p \<in> paths. \<forall>q \<in> paths. q \<in> two_cyclic_set \<and> p \<in> two_cyclic_set \<longrightarrow> p = q"
+proof
+  fix p
+  assume p_in_paths: "p \<in> paths"
+  show "\<forall>q\<in>paths. q \<in> two_cyclic_set \<and> p \<in> two_cyclic_set \<longrightarrow> p = q "
+  proof
+    fix q
+    assume q_in_paths: "q \<in> paths"
+    show "q \<in> two_cyclic_set \<and> p \<in> two_cyclic_set \<longrightarrow> p = q "
+    proof
+      assume q_in_set: "q \<in> two_cyclic_set \<and> p \<in> two_cyclic_set"
+      then have a: "q \<in> two_cyclic_set" and b: " p \<in> two_cyclic_set" by auto
+      show "p = q"
+      proof
+        fix x
+        from b have p_IN: "INPUT(p x) = 1" using two_cyclic_set_def p_in_paths
+          by (metis mem_Collect_eq two_cyclic_path.cases) 
+        from a have q_IN: "INPUT(q x) = 1"  using two_cyclic_set_def p_in_paths
+          by (metis mem_Collect_eq q_in_paths two_cyclic_path.cases)
+        hence equiv_IN:  "INPUT(q x) = INPUT(p x)" using q_IN p_IN by auto
+        from paths_def have  "t(STATE(p x), INPUT(p x)) = (STATE(p (Suc x)), OUT(p x))" using p_in_paths by blast
+        then have p_def: "t(STATE(p x), 1) = (STATE(p (Suc x)), OUT(p x))" using p_IN by simp
+        from paths_def have q_def: "t(STATE(q x), INPUT(q x)) = (STATE(q (Suc x)), OUT(q x))" using q_in_paths by blast
+        then have q_def:  "t(STATE(q x), 1) = (STATE(q (Suc x)), OUT(q x))" using q_IN by simp
+        
+        
+        
+      qed
+    qed
+  qed
+qed
 lemma cyclic_paths_not_empty: "cyclic_paths \<noteq> {}"
 proof
   fix n
@@ -125,16 +163,13 @@ proof
   from 4 0 show "False" by auto
 qed
 
-lemma 45: "\<forall>p \<in> paths. \<forall>i. \<exists>k. t(STATE(p i), k) = (STATE(p (Suc i)), OUT(p i)) \<and> INPUT(p i) > 0 \<longrightarrow> t(STATE(p i), INPUT(p i)) = (STATE(p (Suc i)), OUT(p i))"
-  by simp
-
 lemma stays_in_s_2: "\<forall>p \<in> paths. STATE(p n) = S_1 \<and> INPUT(p n) > 0 \<and> (\<forall>j. j \<in> {n<..<m} \<longrightarrow> INPUT(p j) = 0)  \<and> i \<in> {n<..<m}\<longrightarrow> STATE(p i) = S_2"
 proof
   fix p
   assume base: "p\<in>paths"
   show "STATE (p n) = S_1 \<and> 0 < INPUT (p n) \<and> (\<forall>j. j \<in> {n<..<m} \<longrightarrow> INPUT (p j) = 0) \<and> i \<in> {n<..<m} \<longrightarrow> STATE (p i) = S_2"
   proof (induction i)
-      case 0
+    case 0
       then show ?case
         by simp
     next
@@ -150,58 +185,128 @@ proof
         then show "STATE (p (Suc i)) = S_2"
         proof (cases)
           case 1
-          (*to use IH, one must prove the preconditions, or find a falsity and use False \<longrightarrow> P*)
-          then have "i \<notin> {n<..<m}" using 1 d by simp
-          then have "STATE (p n) = S_1 \<and> 0 < INPUT (p n) \<and> (\<forall>j. j \<in> {n<..<m} \<longrightarrow> INPUT (p j) = 0) \<and> i \<in> {n<..<m} \<longleftrightarrow> False" by blast
-          thus ?thesis 
+          then have 0: "STATE(p i) = S_1" using a by simp
+          from b have 2: "INPUT(p i) > 0" using 1 by simp
+          from paths_def 2 0 have "(S_2, True) = (STATE(p (Suc i)), OUT(p i))"
+            by (smt (verit) base gr0_implies_Suc mem_Collect_eq t.simps(2)) 
+          then have "STATE(p (Suc i)) = S_2" by simp
+          then show ?thesis.
         next
           case 2
-          then have a_2: "STATE (p n) = S_1" 
-          and b_2:" 0 < INPUT (p n)"
-          and c_2: "(\<forall>j. j \<in> {n<..<m} \<longrightarrow> INPUT (p j) = 0)"
-            using LHS by auto
-          (*show i \<in> {n<..<m}*)
-          from d have e_2: "Suc i \<in> {n <..<m}" by auto
-          have "Suc i > Suc n"
-            using d "2" by fastforce
-          then have d_2: "i \<in> {n <..<m}"
-            using d by auto
-          from c_2 d_2 have f: "INPUT(p i) = 0" by blast
-          from a_2 b_2 c_2 d_2 have IH: "STATE(p i) = S_2"
-            using Suc by blast 
-          from c_2 e_2 have "INPUT(p (Suc i)) = 0" by blast
-          then have i_path: "\<exists>k. t(STATE(p i), k) = (STATE(p (Suc i)), OUT(p i))" using paths_def base by blast
-
-          then have "\<exists>k. t(STATE(p i), k) = t(STATE(p i), INPUT(p i))" using c_2 d_2
-            by blast
-          then have "t(STATE(p i), INPUT(p i)) = t(S_2, 0)" using f IH by simp
-          then have "... = (S_2, True)" by simp
-          
-          
-        
-          
+          have a_2: "STATE (p n) = S_1 \<and> 0 < INPUT (p n) \<and> (\<forall>j. j \<in> {n<..<m} \<longrightarrow> INPUT (p j) = 0)" using a b c by simp
+          also have d_2: "i \<in> {n<..<m}"
+            using "2" LHS by force
+          hence IH: "STATE(p i) = S_2"
+          using LHS Suc by fastforce
+          hence "INPUT(p i) = 0" using a_2 d_2 by simp
+          hence "t(STATE(p i), INPUT(p i)) = (STATE(p(Suc i)), OUT(p i))" using paths_def base by blast
+          hence "t(S_2, 0) = (STATE(p(Suc i)), OUT(p i))" using IH
+            by (simp add: \<open>INPUT (p i) = 0\<close>)
+          hence "(STATE(p (Suc i)), OUT(p i)) = (S_2, True)" by simp
+          hence "STATE(p (Suc i)) = S_2" by simp
+          thus ?thesis.  
+        qed
         qed
     qed
   qed
-qed
-
-  
 
 
-lemma "\<forall>p \<in> paths. STATE(p n) = S_1 \<and> INPUT(p n) > 0 \<and> (\<forall>j. j \<in> {n<..<m} \<longrightarrow> INPUT(p j) = 0) \<and> i \<in> {n<..<m} \<longrightarrow> OUT(p i) = True"
+lemma stays_in_s_1: "\<forall>p \<in> paths. STATE(p n) = S_2 \<and> INPUT(p n) > 0 \<and> (\<forall>j. j \<in> {n<..<m} \<longrightarrow> INPUT(p j) = 0)  \<and> i \<in> {n<..<m}\<longrightarrow> STATE(p i) = S_1"
+  proof
+  fix p
+  assume base: "p\<in>paths"
+  show "STATE (p n) = S_2 \<and> 0 < INPUT (p n) \<and> (\<forall>j. j \<in> {n<..<m} \<longrightarrow> INPUT (p j) = 0) \<and> i \<in> {n<..<m} \<longrightarrow> STATE (p i) = S_1"
+  proof (induction i)
+    case 0
+      then show ?case
+        by simp
+    next
+      case (Suc i)
+      show ?case
+      proof
+        assume LHS: "STATE (p n) = S_2 \<and> 0 < INPUT (p n) \<and> (\<forall>j. j \<in> {n<..<m} \<longrightarrow> INPUT (p j) = 0) \<and> Suc i \<in> {n<..<m}"
+        then have a: "STATE (p n) = S_2" 
+        and b: "0 < INPUT (p n)"
+        and c: " (\<forall>j. j \<in> {n<..<m} \<longrightarrow> INPUT (p j) = 0)"
+        and d: "Suc i \<in> {n<..<m}" by auto
+        then consider "Suc i = Suc n" | "Suc i \<noteq> Suc n" by auto
+        then show "STATE (p (Suc i)) = S_1"
+        proof (cases)
+          case 1
+          then have 0: "STATE(p i) = S_2" using a by simp
+          from b have 2: "INPUT(p i) > 0" using 1 by simp
+          from paths_def 2 0 have "(S_1, False) = (STATE(p (Suc i)), OUT(p i))"
+          by (smt (verit) base gr0_implies_Suc mem_Collect_eq t.simps(4)) 
+          then have "STATE(p (Suc i)) = S_1" by simp
+          then show ?thesis.
+        next
+          case 2
+          have a_2: "STATE (p n) = S_2 \<and> 0 < INPUT (p n) \<and> (\<forall>j. j \<in> {n<..<m} \<longrightarrow> INPUT (p j) = 0)" using a b c by simp
+          also have d_2: "i \<in> {n<..<m}"
+            using "2" LHS by force
+          hence IH: "STATE(p i) = S_1"
+          using LHS Suc by fastforce
+          hence "INPUT(p i) = 0" using a_2 d_2 by simp
+          hence "t(STATE(p i), INPUT(p i)) = (STATE(p(Suc i)), OUT(p i))" using paths_def base by blast
+          hence "t(S_1, 0) = (STATE(p(Suc i)), OUT(p i))" using IH
+            by (simp add: \<open>INPUT (p i) = 0\<close>)
+          hence "(STATE(p (Suc i)), OUT(p i)) = (S_1, False)" by simp
+          hence "STATE(p (Suc i)) = S_1" by simp
+          thus ?thesis.  
+        qed
+        qed
+    qed
+  qed
+
+lemma security_s1_to_s2: "\<forall>p \<in> paths. STATE(p n) = S_1 \<and> INPUT(p n) > 0 \<and> (\<forall>j. j \<in> {n<..<m} \<longrightarrow> INPUT(p j) = 0) \<and> i \<in> {n<..<m} \<longrightarrow> OUT(p i) = True"
 proof
-  assume 0: "p \<in> paths"
-  assume 1: "STATE(p n) = S_1 \<and> INPUT(p n) > 0 \<and> (\<forall>j. j \<in> {n<..<m} \<longrightarrow> INPUT(p j) = 0) \<and> i \<in> {n<..<m} "
-  (*show OUT(p i)*)
-  from 0 1 have "\<exists>k. t(STATE(p j), k) = (STATE(p (Suc j)), OUT(p j))" using paths_def by blast
-  then have "t(S_2, 0) = (STATE(p (Suc j)), OUT(p j))"
-    by (metis "0" "1" State.distinct(1) stays_in_s_2)
-  then have "(S_2, True) = (STATE(p (Suc j)), OUT(p j))" by simp
-  then have "OUT(p j) = True" by simp
-  
-lemma lower_bound: "\<forall>p\<in>paths. \<exists>n::nat. m>n \<longrightarrow> (STATE(p n) = S_1) \<longrightarrow> (INPUT(p n) > 0) \<longrightarrow> (INPUT(p m) = 0) \<longrightarrow> (OUTPUT(p m) = True)"
-  by auto
+  fix p
+  assume p_in_paths: "p\<in>paths"
+  show "STATE (p n) = S_1 \<and> 0 < INPUT (p n) \<and> (\<forall>j. j \<in> {n<..<m} \<longrightarrow> INPUT (p j) = 0) \<and> i \<in> {n<..<m} \<longrightarrow> OUT (p i) = True"
+  proof
+    assume LHS: "STATE (p n) = S_1 \<and> 0 < INPUT (p n) \<and> (\<forall>j. j \<in> {n<..<m} \<longrightarrow> INPUT (p j) = 0) \<and> i \<in> {n<..<m}"
+    show "OUT(p i) = True"
+    proof-
+      from LHS have a: "STATE (p n) = S_1" 
+        and b: "0 < INPUT (p n)"
+        and c: " (\<forall>j. j \<in> {n<..<m} \<longrightarrow> INPUT (p j) = 0)"
+        and d: "i \<in> {n<..<m}"
+          by auto
+      from d c have i_input: "INPUT(p i) = 0" by blast
+      from paths_def have "t(STATE(p i), INPUT(p i)) = (STATE(p(Suc i)), OUT(p i))" using p_in_paths by blast
+      then have "t(S_2, 0) = (STATE(p(Suc i)), OUT(p i))" using i_input stays_in_s_2
+          by (metis LHS p_in_paths)
+        then have final: "OUT(p i) = True" by simp
+        then show ?thesis.    
+      qed
+    qed
+  qed
 
+
+lemma security_s2_to_s1: "\<forall>p \<in> paths. STATE(p n) = S_2 \<and> INPUT(p n) > 0 \<and> (\<forall>j. j \<in> {n<..<m} \<longrightarrow> INPUT(p j) = 0) \<and> i \<in> {n<..<m} \<longrightarrow> OUT(p i) = False"
+proof
+  fix p
+  assume p_in_paths: "p \<in> paths"
+  show "STATE(p n) = S_2 \<and> INPUT(p n) > 0 \<and> (\<forall>j. j \<in> {n<..<m} \<longrightarrow> INPUT(p j) = 0) \<and> i \<in> {n<..<m} \<longrightarrow> OUT(p i) = False"
+  proof
+    assume LHS: "STATE(p n) = S_2 \<and> INPUT(p n) > 0 \<and> (\<forall>j. j \<in> {n<..<m} \<longrightarrow> INPUT(p j) = 0) \<and> i \<in> {n<..<m}"
+    show "OUT(p i) = False"
+    proof-
+      from LHS have a: "STATE(p n) = S_2" and b: "INPUT(p n) > 0" and c: "(\<forall>j. j \<in> {n<..<m} \<longrightarrow> INPUT(p j) = 0)" and d:  "i \<in> {n<..<m}" by auto
+      from d c have i_input: "INPUT(p i) = 0" by blast
+      from paths_def have "t(STATE(p i), INPUT(p i)) = (STATE(p(Suc i)), OUT(p i))" using p_in_paths by blast
+      then have "t(S_1, 0) = (STATE(p(Suc i)), OUT(p i))" using i_input stays_in_s_2
+        by (metis LHS p_in_paths stays_in_s_1)
+        then have final: "OUT(p i) = False" by simp
+        then show ?thesis.    
+      qed
+    qed
+  qed
+
+
+
+
+  
 
 
 
